theories/Events/State.v
@@ -68,43 +68,6 @@ Arguments put {S E _}.
 Arguments run_state {S E} [_] _ _.
 
 
-(* ----------------------------------------------------------------------- *)
-(* SAZ: The code from here to <END> below doesn't belong to State.v  it should 
-   go in Prop.v or something like that . *)
-(* todo(gmm): this can be stronger if we allow for a `can_returnE` *)
-Inductive can_return {E : Type -> Type} {t : Type} : itree E t -> t -> Prop :=
-| can_return_Ret {x} : can_return (Ret x) x
-| can_return_Tau {tr x} (_ : can_return tr x) : can_return (Tau tr) x
-| can_return_Vis {u e k} {x: u} {res} (_ : can_return (k x) res)
-  : can_return (Vis e k) res.
-
-(** A propositional "interpreter"
-    This can be useful for non-determinism.
- *)
-Section interp_prop.
-  Context {E F : Type -> Type}.
-
-  Definition eff_hom_prop : Type :=
-    forall t, E t -> itree F t -> Prop.
-
-  CoInductive interp_prop (f : eff_hom_prop) (R : Type)
-  : itree E R -> itree F R -> Prop :=
-  | ipRet : forall x, interp_prop f R (Ret x) (Ret x)
-  | ipVis : forall {T} {e : E T} {e' : itree F T}
-              (k : _ -> itree E R) (k' : T -> itree F R),
-      f _ e e' ->
-      (forall x,
-          can_return e' x ->
-          interp_prop f R (k x) (k' x)) ->
-      interp_prop f R (Vis e k) (ITree.bind e' k')
-  | ipDelay : forall a b, interp_prop f R a b ->
-                     interp_prop f R (Tau a) (Tau b).
-
-End interp_prop.
-Arguments eff_hom_prop _ _ : clear implicits.
-(* <END> -------------------------------------------------------------------- *)
-
-
 (** An extensional stateful handler *)
 Section eff_hom_e.
   Context {E F : Type -> Type}.
